tests/lean/run/simp3.lean
@@ -13,8 +13,6 @@ theorem ex3 (x : Nat) : g (x + 1) = 2 := by simp
 
 theorem ex4 (x : Nat) : (fun x => x + 1) = (fun x => x.succ) := by simp
 
-@[simp] theorem comm (x y : Nat) : x + y = y + x := Nat.addComm ..
-@[simp] theorem addZ (x : Nat) : x + 0 = x := rfl
-@[simp] theorem zAdd (x : Nat) : 0 + x = x := Nat.zeroAdd ..
+@[simp] theorem comm (x y : Nat) : x + y = y + x := Nat.add_comm ..
 
 theorem ex5 (x y : Nat) : (fun x y : Nat => x + 0 + y) = (fun x y : Nat => y + x + 0) := by simp
